Device.v
@@ -1,0 +1,305 @@
+(* Represents an abstract memory deviceice object *)
+Require Import Kami.AllNotations.
+
+Require Import ProcKami.FU.
+Require Import ProcKami.MemOps.
+Require Import ProcKami.MemOpsFuncs.
+Require Import ProcKami.MemRegion.
+
+Require Import StdLibKami.Router.Ifc.
+
+Import ListNotations.
+
+Import BinNat.
+
+Section DeviceIfc.
+  Context {procParams : ProcParams}.
+
+  Inductive PMAAmoClass := AMONone | AMOSwap | AMOLogical | AMOArith.
+
+  Record PMA
+    := {
+        pma_width : nat; (* in bytes *)
+        pma_readable : bool;
+        pma_writeable : bool;
+        pma_executable : bool;
+        pma_misaligned : bool;
+        pma_amo : PMAAmoClass
+      }.
+
+  Definition pmas_default
+    := map
+         (fun x
+          => {|
+              pma_width      := x;
+              pma_readable   := true;
+              pma_writeable  := true;
+              pma_executable := true;
+              pma_misaligned := true;
+              pma_amo        := AMOArith
+            |})
+         [0; 1; 2; 3].
+
+  Definition Req tagK
+    := STRUCT_TYPE {
+         "tag"    :: tagK;
+         "memOp"  :: MemOpCode;
+         "offset" :: PAddr;
+         "data"   :: Data
+       }.
+
+  Definition Res tagK
+    := STRUCT_TYPE {
+         "tag" :: tagK;
+         "res" :: Maybe Data
+       }.
+
+  Record Device
+    := {
+         name : string;
+         io   : bool;
+         pmas : list PMA;
+         deviceFiles: list RegFileBase;
+         deviceRegs: list RegInitT;
+         deviceIfc : forall tagK, DeviceIfc (Req tagK) (Res tagK)
+       }.
+
+  Definition regFiles (devices : list Device)
+    :  list RegFileBase
+    := concat (map deviceFiles devices).
+
+  Definition regs (devices : list Device)
+    := concat (map deviceRegs devices).
+
+  Record RegNames := {
+    deviceBusyRegName : string;
+    deviceReqRegName : string;
+    deviceResRegName : string
+  }. 
+
+  Definition createRegNames
+    (name : string)
+    :  RegNames
+    := {|
+         deviceBusyRegName := @^name ++ "_busy";
+         deviceReqRegName := @^name ++ "_req";
+         deviceResRegName := @^name ++ "_res"
+       |}.
+
+  Class BaseDevice := {
+    regNames : RegNames;
+
+    readReq  : forall ty, PAddr @# ty -> ActionT ty Void;
+    write : forall ty, MemWrite @# ty -> ActionT ty Bool;
+
+    (* Returns the value retrieved by the last read request. *)
+    readRes : forall ty, ActionT ty (Maybe Data);
+  }.
+
+  Definition createRegs tagK
+    (name : string)
+    :  list RegInitT
+    := let names : RegNames := createRegNames name in
+       makeModule_regs (Register (@deviceBusyRegName names): Bool <- Default ++
+                        Register (@deviceReqRegName names): Maybe (Req tagK) <- Default ++
+                        RegisterU (@deviceResRegName names): Maybe Data)%kami.
+
+  Section ty.
+    Context (baseDevice: BaseDevice).
+    Variable ty : Kind -> Type.
+
+    Local Open Scope kami_expr.
+    Local Open Scope kami_action.
+
+    Local Definition deviceIsRead
+      :  MemOpCode @# ty -> ActionT ty Bool
+      := applyMemOp
+           memOps
+           (fun memOp
+             => Ret
+                  $$(orb
+                    (isMemRegValueFn (memOpRegValue memOp))
+                    (isMemWriteValueFn (memOpWriteValue memOp)))).
+
+    Local Definition deviceRead
+      (code : MemOpCode @# ty)
+      (addr : PAddr @# ty)
+      :  ActionT ty Void
+      := LETA isRead : Bool <- deviceIsRead code;
+         If #isRead
+           then readReq addr;
+         Retv.
+
+    Local Definition deviceWriteValue
+      (code : MemOpCode @# ty)
+      (memData : Data @# ty)
+      (regData : Data @# ty)
+      :  ActionT ty (Maybe Data)
+      := applyMemOp
+           memOps
+           (fun memOp
+             => match memOpWriteValue memOp return ActionT ty (Maybe Data) with
+                | memWriteValueFn f
+                  => LETA result : Data
+                       <- convertLetExprSyntax_ActionT
+                            (f ty regData memData);
+                     Ret (Valid #result : Maybe Data @# ty)
+                | memWriteValueStore
+                  => Ret (Valid regData)
+                | memWriteValueNone
+                  => Ret (Invalid : Maybe Data @# ty)
+                end)
+           code.
+
+    Local Definition deviceWriteMask
+      :  MemOpCode @# ty -> ActionT ty DataMask
+      := applyMemOp
+           memOps
+           (fun memOp
+             => Ret (getMask (memOpSize memOp) ty)).
+
+    Local Definition deviceWrite
+      (addr : PAddr @# ty)
+      (writeMask : DataMask @# ty)
+      (writeData : Maybe Data @# ty)
+      :  ActionT ty Bool
+      := If writeData @% "valid"
+           then 
+             LET writeReq
+               :  MemWrite
+               <- STRUCT {
+                    "addr" ::= addr;
+                    "data" ::= unpack (Array Rlen_over_8 (Bit 8)) (writeData @% "data");
+                    "mask" ::= writeMask
+                  } : MemWrite @# ty;
+             write #writeReq
+           else Ret $$true
+           as result;
+         Ret #result.
+
+    Local Definition deviceRegValue
+      (code : MemOpCode @# ty)
+      (memData : Data @# ty)
+      :  ActionT ty (Maybe Data)
+      := applyMemOp
+           memOps
+           (fun memOp
+             => match memOpRegValue memOp return ActionT ty (Maybe Data) with
+                  | memRegValueFn f
+                    => LETA result : Data <- convertLetExprSyntax_ActionT (f ty memData);
+                       Ret (Valid #result : Maybe Data @# ty)
+                  | memRegValueNone
+                    => Ret (Invalid : Maybe Data @# ty)
+                  end)
+           code.
+
+    Definition deviceSendReqFn tagK
+      (req : ty (Req tagK))
+      :  ActionT ty Bool
+      := Read busy : Bool <- deviceBusyRegName regNames;
+         Write (deviceBusyRegName regNames) : Bool <- $$true;
+         If !#busy
+           then deviceRead (#req @% "memOp") (#req @% "offset");
+         Read currReq
+           :  Maybe (Req tagK)
+           <- deviceReqRegName regNames;
+         Write (deviceReqRegName regNames)
+           :  Maybe (Req tagK)
+           <- IF #busy
+                then #currReq
+                else Valid #req;
+         System [
+           DispString _ "[Device.deviceSendReqFn] req accepted: ";
+           DispHex (!#busy);
+           DispString _ "\n";
+           DispString _ "[Device.deviceSendReqFn] req: ";
+           DispHex #req;
+           DispString _ "\n"
+         ];
+         Ret !#busy.
+
+    (*
+      Reads the value returned by the last read request sent to the
+      deviceice; computes a register result, and memory
+      write value, using the current deviceice request and most recent
+      memory read result; attempts to write the memory write value
+      to memory; and returns the computed register result value.
+
+      * Invalid - retry
+      * Valid Invalid - the memory operation succeeded, no
+        register update
+      * Valid Valid DATA - the memory operation succeeded, data
+        contains the register update value.
+    *)
+    Definition deviceGetResFn tagK
+      :  ActionT ty (Maybe (Res tagK))
+      := Read req : Maybe (Req tagK) <- deviceReqRegName regNames;
+         System [
+           DispString _ "[deviceGetResFn] request in buffer:";
+           DispHex #req;
+           DispString _ "\n"
+         ];
+         If #req @% "valid"
+           then
+             System [
+               DispString _ "[deviceGetResFn] we have a valid request in buffer.\n"
+             ];
+             LETA memData : Maybe Data <- readRes ty;
+             System [
+               DispString _ "[Device.deviceGetResFn] memData: ";
+               DispHex #memData;
+               DispString _ "\n"
+             ];
+             LETA writeData
+               :  Maybe Data
+               <- deviceWriteValue (#req @% "data" @% "memOp") (#memData @% "data") (#req @% "data" @% "data");
+             LETA writeMask
+               :  DataMask
+               <- deviceWriteMask (#req @% "data" @% "memOp");
+             LETA writeSucceeded
+               :  Bool
+               <- deviceWrite (#req @% "data" @% "offset") #writeMask #writeData;
+             LETA regData
+               :  Maybe Data
+               <- deviceRegValue (#req @% "data" @% "memOp") (#memData @% "data");
+             LETA hasLoad
+               :  Bool
+               <- memOpHasLoad memOps (#req @% "data" @% "memOp");
+             Write (deviceReqRegName regNames)
+               :  Maybe (Req tagK)
+               <- Invalid;
+             Write deviceBusyRegName regNames
+               :  Bool
+               <- $$false;
+             LET result
+               :  (Res tagK)
+               <- STRUCT {
+                    "tag" ::= #req @% "data" @% "tag";
+                    "res" ::= #regData
+                  } : (Res tagK) @# ty;
+             Ret
+               (IF #writeSucceeded && #hasLoad
+                 then ((Valid #result) : Maybe (Res tagK) @# ty)
+                 else (Invalid : Maybe (Res tagK) @# ty))
+           else
+             Ret (Invalid : Maybe (Res tagK) @# ty)
+           as res;
+         System [
+           DispString _ "[Device.deviceGetResFn] res: ";
+           DispHex #res;
+           DispString _ "\n"
+         ];
+         Ret #res.
+
+    Local Close Scope kami_action.
+    Local Close Scope kami_expr.
+  End ty.
+
+  Record DeviceTree
+    := {
+        devices : list Device;
+        memTable : list (@MemTableEntry (length devices));
+        memTableIsValid : (@memRegions (length devices) memTable) <> []
+      }.
+
+End DeviceIfc.
