MemOpsFuncs.v
@@ -1,0 +1,128 @@
+(* This module defines the memory operations semantics table. *)
+Require Import Kami.AllNotations.
+Require Import ProcKami.FU.
+
+Import ListNotations.
+
+Section memOpsFuncs.
+  Context {procParams : ProcParams}.
+
+  Local Open Scope kami_expr.
+
+  (* specifies the value stored in the destination register by a memory operation. *)
+  Inductive MemRegValue
+    := memRegValueFn : (forall ty, Data @# ty -> Data ## ty) -> MemRegValue
+    |  memRegValueNone.
+
+  Definition isMemRegValueFn (x : MemRegValue) : bool
+    := match x with
+       | memRegValueFn _ => true
+       | _ => false
+       end.
+
+  (* specifies the value written to memory by a memory operation. *)
+  Inductive MemWriteValue : Type
+    := memWriteValueFn : (forall ty, Data @# ty -> Data @# ty -> Data ## ty) -> MemWriteValue
+    |  memWriteValueStore (* write register value *)
+    |  memWriteValueNone.
+
+  Definition isMemWriteValueFn (x : MemWriteValue) : bool
+    := match x with
+       | memWriteValueFn _ => true
+       | _ => false
+       end.
+
+  Record MemOp := {
+    memOpName : MemOpName;
+    memOpCode : nat;
+    memOpSize : nat;
+    memOpRegValue : MemRegValue;
+    memOpWriteValue : MemWriteValue
+  }.
+
+  Definition getMask (size: nat) ty
+    :  DataMask @# ty
+    := unpack DataMask
+         ($(Nat.pow 2 (Nat.pow 2 size) - 1)).
+
+  Section memOps.
+    Variable memOps : list MemOp.
+
+    Definition applyMemOpByName
+      (t : Type)
+      (f : MemOp -> t)
+      (default : t)
+      (name : MemOpName)
+      :  t
+      := match find (fun memOp => memOpNameEqb name (memOpName memOp)) memOps with
+         | None => default
+         | Some memOp => f memOp
+         end.
+
+    Section ty.
+      Variable ty : Kind -> Type.
+
+      Definition getMemOpCode
+        :  MemOpName -> MemOpCode @# ty
+        := applyMemOpByName
+             (fun memOp => $(memOpCode memOp) : MemOpCode @# ty)
+             $0.
+
+      Local Open Scope kami_action.
+
+      Definition applyMemOp
+        (k : Kind)
+        (f : MemOp -> ActionT ty k)
+        (code : MemOpCode @# ty)
+        :  ActionT ty k
+        := LETA result
+             :  Maybe k
+             <- utila_acts_find_pkt
+                  (map
+                    (fun memOp
+                      => If code == $(memOpCode memOp)
+                           then
+                             LETA result : k <- f memOp;
+                             Ret (Valid #result : Maybe k @# ty)
+                           else
+                             Ret (Invalid : Maybe k @# ty)
+                           as result;
+                         Ret #result)
+                    memOps);
+           Ret (#result @% "data").
+
+      (* stores excluding AMOs that do not generate write backs. *)
+      Definition memOpHasLoad
+        :  MemOpCode @# ty -> ActionT ty Bool
+        := applyMemOp
+             (fun memOp => Ret $$(isMemRegValueFn (memOpRegValue memOp))).
+
+      Local Close Scope kami_action.
+
+      Section func_units. 
+        Variable func_units : list FUEntry.
+
+        Local Open Scope kami_action.
+
+        Definition applyMemInst
+          (k : Kind)
+          (f : forall t u, InstEntry t u -> MemOp -> k ## ty)
+          :  FuncUnitId func_units @# ty -> InstId func_units @# ty -> k ## ty
+          := applyInst
+               (fun t u inst
+                 => match optMemParams inst with
+                    | Some name
+                      => match find (fun memOp => memOpNameEqb name (memOpName memOp)) memOps with
+                         | Some memOp => f t u inst memOp
+                         | None => RetE $$(getDefaultConst k) (* impossible case. *)
+                         end
+                    | None => RetE $$(getDefaultConst k) (* impossible case. *)
+                    end).
+
+        Local Close Scope kami_action.
+
+      End func_units.
+    End ty.
+  End memOps.
+  Local Close Scope kami_expr.
+End memOpsFuncs.
