MemRegion.v
@@ -1,0 +1,167 @@
+(*
+  This module defines the physical memory interface.
+*)
+Require Import Kami.AllNotations.
+
+Require Import ProcKami.FU.
+Require Import ProcKami.MemOps.
+
+
+
+
+
+Import ListNotations.
+
+Import BinNat.
+
+Section pmem.
+  Context {procParams: ProcParams}.
+  Context (numDevices : nat).
+  Variable ty: Kind -> Type.
+  
+  Record MemTableEntry
+    := {
+        addr  : N;
+        width : N;
+        device : Fin.t numDevices
+      }.
+
+  Record MemRegion
+    := {
+         mem_region_addr : N;
+         mem_region_width : N;
+         mem_region_device_offset : N; (* device offset *)
+         mem_region_device : option (Fin.t numDevices)
+       }.
+
+  Local Definition list_sum : list N -> N := fold_right N.add 0%N.
+
+  (* memory regions from largest start address to smallest start address *)
+  Local Definition mem_table_regions
+    :  list MemTableEntry -> option (N * list MemRegion)%type
+    := fold_right
+         (fun x acc
+           => match acc with
+                | None => None
+                | Some (end_addr, regions)
+                  => let next_end_addr := (x.(addr) + x.(width))%N in
+                     let gap_addr := list_sum (map mem_region_width regions) in
+                     let gap_width := (x.(addr) - end_addr)%N in
+                     let device_region
+                       := {|
+                            mem_region_addr := (gap_addr + gap_width)%N;
+                            mem_region_width := x.(width);
+                            mem_region_device_offset
+                              := list_sum
+                                   (map mem_region_width
+                                     (filter
+                                       (fun prev_region
+                                         => fromOption
+                                              (option_map
+                                                (Fin.eqb x.(device))
+                                                (mem_region_device prev_region))
+                                              false)
+                                       regions));
+                            mem_region_device := Some x.(device)
+                          |} in
+                     if (end_addr <? x.(addr))%N
+                     then
+                       Some (next_end_addr,
+                         device_region ::
+                         {|
+                           mem_region_addr := gap_addr;
+                           mem_region_width := gap_width;
+                           mem_region_device_offset := 0%N; (* no device offset *)
+                           mem_region_device := None
+                         |} ::
+                         regions)
+                     else
+                       if (end_addr =? x.(addr))%N
+                       then Some (next_end_addr, device_region :: regions)
+                       else None
+                end)
+         (Some (0%N, [])).
+
+  (*
+    Accepts three arguments: [f], a function that accepts a memory
+    table entry and returns its starting address as an integer value;
+    [x], a memory table entry; and [ys], a list of memory table entries;
+    and inserts [x] into [ys] so that every preceeding element in the
+    resulting list has a smaller starting address than [x].
+  *)
+  Local Fixpoint mem_table_insert (A : Type) (f : A -> N) (x : A) (ys : list A)
+    :  list A
+    := match ys with
+       | [] => [x]
+       | y0 :: ys
+         => if (f x <? f y0)%N
+            then y0 :: (mem_table_insert f x ys)
+            else x :: y0 :: ys
+       end.
+
+  (*
+    Accepts a list of memory table entries, [xs], and sorts them
+    in ascending order of starting address.
+  *)
+  Local Definition mem_table_sort
+    :  list MemTableEntry -> list MemTableEntry
+    := fold_right
+         (mem_table_insert
+           addr)
+         [].
+
+  Definition memRegions
+    (memTable : list MemTableEntry)
+    := match mem_table_regions (mem_table_sort memTable) with
+         | Some (_, regions) => regions
+         | _ => []
+         end.
+
+  Local Definition option_eqb (A : Type) (H : A -> A -> bool) (x y : option A) : bool
+    :=  match x, y with
+         | None, None => true
+         | Some n, Some m => H n m
+         | _, _ => false
+        end.
+
+  Local Open Scope kami_expr.
+  Local Open Scope kami_action.
+
+  Section ty.
+
+    Local Definition mem_region_match
+      (* (region_addr : N) *)
+      (region : MemRegion)
+      (paddr : PAddr @# ty)
+      :  Bool @# ty
+      := let region_addr := mem_region_addr region in
+         (($$(NToWord PAddrSz region_addr) <= paddr) &&
+         (paddr < $$(NToWord PAddrSz (region_addr + mem_region_width region)%N))).
+
+    Definition memRegionApply
+      (k : Kind)
+      (paddr : FU.PAddr @# ty)
+      (f : MemRegion -> PAddr @# ty -> ActionT ty k)
+      (memRegions : list MemRegion)
+      :  ActionT ty (Maybe k)
+      := utila_acts_find_pkt
+           (map
+             (fun region
+               => If mem_region_match region paddr
+                    then
+                      LETA result
+                        <- f region
+                             ((paddr - $$(NToWord PAddrSz (mem_region_addr region))) +
+                              $$(NToWord PAddrSz (mem_region_device_offset region)));
+                      Ret (Valid #result : Maybe k @# ty)
+                    else Ret Invalid
+                    as result;
+                  Ret #result)
+             memRegions).
+
+  End ty.
+
+  Local Close Scope kami_action.
+  Local Close Scope kami_expr.
+
+End pmem.
