Pipeline/Impl.v
@@ -1,0 +1,422 @@
+Require Import Kami.AllNotations.
+
+Require Import StdLibKami.Fifo.Ifc.
+
+Require Import ProcKami.Pipeline.Mem.Ifc.
+Require Import ProcKami.Pipeline.Mem.Impl.
+
+Require Import ProcKami.Pipeline.Decoder.
+Require Import ProcKami.Pipeline.RegReader.
+Require Import ProcKami.Pipeline.InputXform.
+Require Import ProcKami.Pipeline.Executer.
+Require Import ProcKami.Pipeline.Commit.
+Require Import ProcKami.Pipeline.ConfigReader.
+
+Require Import ProcKami.Pipeline.Ifc.
+
+Require Import ProcKami.MemOps.
+Require Import ProcKami.MemOpsFuncs.
+
+Require Import ProcKami.FU.
+Require Import ProcKami.Device.
+
+Section Impl.
+  Context {procParams: ProcParams}.
+  Context (func_units : list FUEntry).
+  Context (deviceTree: @DeviceTree procParams).
+  Context (memParams: @Mem.Ifc.Params).
+
+  Local Definition CommitPkt := (STRUCT_TYPE {
+                                     "incompletePc" :: Maybe FU.VAddr ;
+                                     "execCxt"    :: ExecContextPkt ;
+                                     "execUpd"    :: ExecUpdPkt ;
+                                     "exception"  :: Maybe Exception })%kami_expr.
+
+  Local Instance tokenFifoParams
+    :  Fifo.Ifc.Params
+    := {| Fifo.Ifc.name := @^"tokenFifo";
+          Fifo.Ifc.k := Void;
+          Fifo.Ifc.size := 1;
+       |}.
+
+  Local Instance fetchAddrExceptionFifoParams
+    :  Fifo.Ifc.Params
+    := {| Fifo.Ifc.name := @^"fetchAddrExceptionFifo";
+          Fifo.Ifc.k := Maybe Exception;
+          Fifo.Ifc.size := 1;
+       |}.
+
+  Local Instance fetchInstExceptionFifoParams
+    :  Fifo.Ifc.Params
+    := {| Fifo.Ifc.name := @^"fetchInstExceptionFifo";
+          Fifo.Ifc.k := Maybe Exception;
+          Fifo.Ifc.size := 2 ^ fetcherLgSize;
+       |}.
+
+  Local Instance decExecFifoParams
+    :  Fifo.Ifc.Params
+    := {| Fifo.Ifc.name := @^"decExecFifo";
+          Fifo.Ifc.k := CommitPkt;
+          Fifo.Ifc.size := 1;
+       |}.
+
+  Local Definition tokenFifo: @Fifo.Ifc.Ifc tokenFifoParams.
+    refine (@Fifo.Impl.impl _ {| Fifo.Impl.sizePow2 := _ ;
+                                 Fifo.Impl.regArray := @RegArray.Impl.impl _ |}).
+    abstract auto.
+  Defined.
+
+  Local Definition fetchAddrExceptionFifo: @Fifo.Ifc.Ifc fetchAddrExceptionFifoParams.
+    refine (@Fifo.Impl.impl _ {| Fifo.Impl.sizePow2 := _ ;
+                                 Fifo.Impl.regArray := @RegArray.Impl.impl _ |}).
+    abstract auto.
+  Defined.
+
+  Local Definition decExecFifo: @Fifo.Ifc.Ifc decExecFifoParams.
+    refine (@Fifo.Impl.impl _ {| Fifo.Impl.sizePow2 := _ ;
+                                 Fifo.Impl.regArray := @RegArray.Impl.impl _ |}).
+    abstract auto.
+  Defined.
+
+  Local Definition fetchInstExceptionFifo: @Fifo.Ifc.Ifc fetchInstExceptionFifoParams.
+    refine (@Fifo.Impl.impl _ {| Fifo.Impl.sizePow2 := _ ;
+                                 Fifo.Impl.regArray := @RegArray.Impl.impl _ |}).
+    abstract (simpl; rewrite Natlog2_up_pow2; auto).
+  Defined.
+
+  Section memInterfaceSizeParams.
+    Local Open Scope kami_action.
+    Local Open Scope kami_expr.
+
+    Local Definition memCallback ty
+               (res: ty (@MemResp _ memParams))
+      :  ActionT ty Void
+      := System [
+           DispString _ "[memCallback] res: ";
+           DispHex #res;
+           DispString _ "\n"
+         ];
+         LETA oldOptCommit : Maybe CommitPkt <- @Fifo.Ifc.first _ decExecFifo _;
+         LET wb : RoutedReg <- STRUCT {
+                                 "tag" ::= (IF #oldOptCommit @% "data" @% "execCxt" @% "memHints" @% "data" @% "isFrd"
+                                             then $FloatRegTag
+                                             else $IntRegTag);
+                                 "data"  ::= #res @% "res" @% "data"
+                               };
+         LET newUpdatePkt
+           :  ExecUpdPkt
+           <- IF #res @% "res" @% "valid"
+                then #oldOptCommit @% "data" @% "execUpd" @%["val1" <- Valid #wb]
+                else #oldOptCommit @% "data" @% "execUpd";
+         LET commitPkt
+           :  CommitPkt
+           <- #oldOptCommit @% "data" @%["execUpd" <- #newUpdatePkt];
+         LETA cxtCfg: ContextCfgPkt <- readConfig _;
+         System [
+           DispString _ "[memCallback] commit pkt: ";
+           DispHex #commitPkt;
+           DispString _ "\n"
+         ];
+         LETA _ <- commit #cxtCfg (#commitPkt @% "execCxt") (#commitPkt @% "execUpd") (#commitPkt @% "exception");
+         LETA _ <- @Fifo.Ifc.deq _ decExecFifo _;
+         LET  tokenFifoVal : Void <- $$(getDefaultConst Void);
+         LETA _ <- @Fifo.Ifc.enq _ tokenFifo _ tokenFifoVal;
+         Retv.
+
+    Local Close Scope kami_expr.
+    Local Close Scope kami_action.
+  End memInterfaceSizeParams.
+  
+  Local Definition mem := @Mem.Impl.impl  _ deviceTree _ memCallback.
+
+  Section ty.
+    Variable ty: Kind -> Type.
+
+    Local Open Scope kami_action.
+    Local Open Scope kami_expr.
+
+    Local Definition tokenStartRule: ActionT ty Void :=
+      Read initReg <- @^"initReg";
+      If !#initReg
+      then (
+        System [
+          DispString _ "[tokenStart]\n"
+        ];
+        LET tokenVal: Void <- $$(getDefaultConst Void);
+        LETA _ <- @Fifo.Ifc.enq _ tokenFifo _ tokenVal;
+        Write @^"initReg" <- $$true;
+        Retv );
+      Retv.
+
+    Local Definition sendPcRule: ActionT ty Void :=
+      LETA cxtCfg: ContextCfgPkt <- readConfig _;
+      LETA isEmpty <- @Fifo.Ifc.isEmpty _ tokenFifo _;
+      LETA isFull <- @fetcherIsFull procParams deviceTree _ mem ty;
+      Read pc : FU.VAddr <- @^"pc";
+      System [
+        DispString _ "[sendPcRule] fifo is empty: ";
+        DispHex #isEmpty;
+        DispString _ "\n";
+        DispString _ "[sendPcRule] fetcher is full: ";
+        DispHex #isFull;
+        DispString _ "\n"
+      ];
+      If !#isEmpty && !#isFull
+      then (
+        LETA optPAddrDevOffsetException
+          :  Maybe (PktWithException (@PAddrDevOffset _ deviceTree))
+          <- @memTranslate _ _ _ mem _ #cxtCfg $VmAccessInst (getMemOpCode memOps _ Lw) #pc;
+        System [
+          DispString _ "[sendPcRule] optPAddrDevOffsetException: ";
+          DispHex #optPAddrDevOffsetException;
+          DispString _ "\n"
+        ];
+        If #optPAddrDevOffsetException @% "valid"
+        then (
+          LET inReq : PAddrDevOffsetVAddr deviceTree <- STRUCT { "memReq" ::= #optPAddrDevOffsetException @% "data" @% "fst" ;
+                                                                 "vaddr" ::= #pc } ;
+          LET req <- STRUCT { "inReq" ::= #inReq ;
+                              "sendReq?" ::= !(#optPAddrDevOffsetException @% "data" @% "snd" @% "valid") };
+          LETA accepted : Bool <- @Mem.Ifc.fetcherSendAddr _ _ _ mem ty req;
+          If #accepted
+          then (
+            LET val : Maybe Exception <- (#optPAddrDevOffsetException @% "data" @% "snd");
+            LETA _ <- @Fifo.Ifc.enq _ fetchAddrExceptionFifo _ val;
+            LETA _ <- @Fifo.Ifc.deq _ tokenFifo _;
+            Retv );
+          Retv );
+        Retv);
+      Retv.
+
+    Local Definition transferMmuFetchExceptionRule: ActionT ty Void :=
+      LETA optPAddrException <- @Fifo.Ifc.first _ fetchAddrExceptionFifo _;
+      LETA isFull <- @Fifo.Ifc.isFull _ fetchInstExceptionFifo _;
+      System [
+        DispString _ "[transferMmuFetchExceptionRule] isFull: ";
+        DispHex #isFull;
+        DispString _ "\n";
+        DispString _ "[transferMmuFetchExceptionRule] optPAddrException: ";
+        DispHex #optPAddrException;
+        DispString _ "\n"
+      ];
+      If (!#isFull && #optPAddrException @% "valid")
+      then (
+        System [
+          DispString _ "[transferMmuFetchExceptionRule]\n"
+        ];
+        LETA _ <- @Fifo.Ifc.deq _ fetchAddrExceptionFifo _;
+        LET pAddrException <- #optPAddrException @% "data";    
+        @Fifo.Ifc.enq _ fetchInstExceptionFifo _ pAddrException
+      );
+      Retv.
+
+    Local Definition decodeExecRule: ActionT ty Void :=
+      LETA optInstException : Maybe (Maybe Exception) <- @Fifo.Ifc.first _ fetchInstExceptionFifo _;
+      LETA isFull <- @Fifo.Ifc.isFull _ decExecFifo _;
+      LETA fetchInst: Maybe FetchOutput <- @Mem.Ifc.fetcherFirst _ _ _ mem _;
+      System [
+        DispString _ "[decodeExecRule] FetchInst: \n";
+        DispHex #fetchInst;
+        DispString _ "\n";
+        DispString _ "[decodeExecRule] Exception: ";
+        DispHex #optInstException;
+        DispString _ "\n";
+        DispString _ "[decodeExecRule] isFull: ";
+        DispHex #isFull;
+        DispString _ "\n"
+        ];
+      If (!#isFull && #optInstException @% "valid" && #fetchInst @% "valid")
+      then (
+        LETA context: ContextCfgPkt <- readConfig _;
+        LET incompPc: Maybe FU.VAddr <- STRUCT { "valid" ::= #fetchInst @% "data" @% "notComplete?" ;
+                                               "data"  ::= #fetchInst @% "data" @% "vaddr"};
+        If (#incompPc @% "valid" || #optInstException @% "data" @% "valid") (* I.A. fetch incomplete or exception. we need to fetch again. *)
+        then (
+          LET enqVal : CommitPkt <- STRUCT { "incompletePc" ::= #incompPc ;
+                                             "execCxt"    ::= $$(getDefaultConst ExecContextPkt) ;
+                                             "execUpd"    ::= $$(getDefaultConst ExecUpdPkt);
+                                             "exception"  ::= (#optInstException @% "data": Maybe Exception @# ty) };
+          System [
+            DispString _ "[decodeExecRule] Incomplete\n"
+            ];
+          LETA _ <- @Fifo.Ifc.enq _ decExecFifo _ enqVal;
+          LETA _ <- @Fifo.Ifc.deq _ fetchInstExceptionFifo _;
+          LETA _ <- @Mem.Ifc.fetcherDeq _ _ _ mem _;
+          Retv )
+        else ( (* I.B. fetch complete and no exception. *)
+          LET fetchPkt: FetchPkt <- STRUCT {
+                                        "pc"             ::= #fetchInst @% "data" @% "vaddr" ;
+                                        "inst"           ::= #fetchInst @% "data" @% "inst" ;
+                                        "compressed?"    ::= #fetchInst @% "data" @% "compressed?" ;
+                                        "exceptionUpper" ::= #fetchInst @% "data" @% "errUpper?" };
+          System [
+            DispString _ "[decodeExecRule] fetch pkt: ";
+            DispHex #fetchPkt;
+            DispString _ "\n"
+          ];
+          LETA decoderPkt <- decoderWithException #context (STRUCT { "fst" ::= #fetchPkt;
+                                                                     "snd" ::= #optInstException @% "data"});
+          System [
+            DispString _ "[decodeExecRule] decoder pkt: ";
+            DispHex #decoderPkt;
+            DispString _ "\n"
+          ];
+          LETA execContextPkt <-
+            readerWithException
+              (func_units := func_units) (#fetchInst @% "data" @% "vaddr") #context #decoderPkt (#fetchPkt @% "compressed?") (#fetchPkt @% "exceptionUpper");
+          System [
+            DispString _ "[decodeExecRule] execute context pkt: ";
+            DispHex #execContextPkt;
+            DispString _ "\n"
+          ];
+          LETA inputPkt <- inputXformWithException #context (#decoderPkt @% "fst") #execContextPkt;
+          System [
+            DispString _ "[decodeExecRule] input pkt: ";
+            DispHex #inputPkt;
+            DispString _ "\n"
+          ];
+          LETA execUpdPkt <- execWithException #inputPkt;
+          System [
+            DispString _ "[decodeExecRule] execute update pkt: ";
+            DispHex #execUpdPkt;
+            DispString _ "\n"
+          ];
+          LET enqVal: CommitPkt <- STRUCT { "incompletePc" ::= #incompPc ;
+                                            "execCxt"      ::= #execContextPkt @% "fst" ;
+                                            "execUpd"      ::= #execUpdPkt @% "fst";
+                                            "exception"    ::= #execUpdPkt @% "snd" };
+          If (#execContextPkt @% "fst" @% "memHints" @% "valid" (* Memory *)
+              && #execUpdPkt @% "fst" @% "val2" @% "valid" (* Not failed Store Conditional - could be other reasons *)
+              && !(#execUpdPkt @% "snd" @% "valid")) (* No Exception *)
+          then (
+            System [
+              DispString _ "[decodeExecRule] sending request to translate memory request addr.\n"
+            ];
+            LET vaddr: FU.VAddr <- xlen_sign_extend Xlen (#context @% "xlen") (#execUpdPkt @% "fst" @% "val2" @% "data" @% "data" : Bit Rlen @# ty);
+            LETA mmuResp: Maybe (PktWithException (PAddrDevOffset deviceTree)) <- @memTranslate _ _ _ mem _  #context
+                                                                                                (IF #execContextPkt @% "fst" @% "memHints" @% "data" @% "isSAmo"
+                                                                                                 then $VmAccessSAmo
+                                                                                                 else $VmAccessLoad)
+                                                                                                (#execContextPkt @% "fst" @% "memHints" @% "data" @% "memOp")
+                                                                                                #vaddr;
+            System [
+              DispString _ "[decodeExecRule] memory request MMU res: ";
+              DispHex #mmuResp;
+              DispString _ "\n"
+            ];
+            If #mmuResp @% "valid" (* TLB Hit *)
+            then (
+              If #mmuResp @% "data" @% "snd" @% "valid" (* TLB exception *)
+              then (
+                LET newEnqVal <- #enqVal @%[ "exception" <- #mmuResp @% "data" @% "snd"];
+                LETA _ <- @Fifo.Ifc.enq _ decExecFifo _ newEnqVal;
+                LETA _ <- @Fifo.Ifc.deq _ fetchInstExceptionFifo _;
+                LETA _ <- @Mem.Ifc.fetcherDeq _ _ _ mem _;
+                Retv )
+              else ( (* TLB no exception *)
+                LET memReq: MemReq deviceTree <- STRUCT { "dtag" ::= #mmuResp @% "data" @% "fst" @% "dtag" ;
+                                                          "offset" ::= #mmuResp @% "data" @% "fst" @% "offset" ;
+                                                          "paddr" ::= #mmuResp @% "data" @% "fst" @% "paddr" ;
+                                                          "memOp" ::= #execContextPkt @% "fst" @% "memHints" @% "data" @% "memOp" ;
+                                                          "data" ::= #execUpdPkt @% "fst" @% "val1" @% "data" @% "data"};
+                LET memUnitMemReq: MemUnitMemReq deviceTree <- STRUCT { "tag" ::= $0;
+                                                                        "req" ::= #memReq };
+                LETA accepted: Bool <- @sendMemUnitMemReq _ _ _ mem _ memUnitMemReq;
+                System [
+                  DispString _ "[decodeExecRule] memory unit req accepted: ";
+                  DispHex #accepted;
+                  DispString _ "\n"
+                ];
+                If #accepted (* Request accepted *)
+                then (
+                  LETA _ <- @Fifo.Ifc.enq _ decExecFifo _ enqVal;
+                  LETA _ <- @Fifo.Ifc.deq _ fetchInstExceptionFifo _ ;
+                  LETA _ <- @Mem.Ifc.fetcherDeq _ _ _ mem _;
+                  Retv ) ;
+                Retv );
+              Retv );
+            Retv )
+          else ( (* Not memory *)
+            LETA _ <- @Fifo.Ifc.enq _ decExecFifo _ enqVal;
+            LETA _ <- @Fifo.Ifc.deq _ fetchInstExceptionFifo _;
+            LETA _ <- @Mem.Ifc.fetcherDeq _ _ _ mem _;
+            Retv );
+          Retv );
+        Retv );
+      Retv.
+
+           (* Exceptions takes more preference *)
+    Local Definition commitRule: ActionT ty Void :=
+      Read isWfi : Bool <- @^"isWfi";
+      LETA optCommit <- @Fifo.Ifc.first _ decExecFifo _;
+      LETA context: ContextCfgPkt <- readConfig _;
+      If #optCommit @% "valid" && !#isWfi 
+      then (
+        System [
+          DispString _ "[commitRule] optCommit: ";
+          DispHex #optCommit;
+          DispString _ "\n"
+        ];
+        LETA hasLoad <- memOpHasLoad memOps (#optCommit @% "data" @% "execCxt" @% "memHints" @% "data" @% "memOp");
+        If #optCommit @% "data" @% "incompletePc" @% "valid"
+        then (
+          Write @^"pc" <- (#optCommit @% "data" @% "incompletePc" @% "data");
+          LETA _ <- @Fifo.Ifc.deq _ decExecFifo _;
+          LET  tokenFifoVal : Void <- $$(getDefaultConst Void);
+          LETA _ <- @Fifo.Ifc.enq _ tokenFifo _ tokenFifoVal;
+          Retv )
+        else (
+          If ((#optCommit @% "data" @% "exception" @% "valid") ||
+              !((#optCommit @% "data" @% "execCxt" @% "memHints" @% "valid") && #hasLoad))
+          then (
+            LETA newPc <- commit #context (#optCommit @% "data" @% "execCxt") (#optCommit @% "data" @% "execUpd")
+                                 (#optCommit @% "data" @% "exception");
+            Write @^"pc" <- #newPc;
+            LETA _ <- @Fifo.Ifc.deq _ decExecFifo _;
+            LET  tokenFifoVal : Void <- $$(getDefaultConst Void);
+            LETA _ <- @Fifo.Ifc.enq _ tokenFifo _ tokenFifoVal;
+            Retv );
+          Retv );
+        Retv );
+      Retv.
+
+    Local Close Scope kami_expr.
+    Local Close Scope kami_action.
+  End ty.
+
+  Definition ArbiterTag := @Mem.Impl.ArbiterTag _ deviceTree _ memCallback.
+  
+  Definition impl
+    :  Ifc
+    := {|
+         Pipeline.Ifc.regs
+           := [
+                (@^"initReg", existT RegInitValT (SyntaxKind Bool) (Some (SyntaxConst (ConstBool false))));
+                (@^"pc", existT RegInitValT (SyntaxKind (Bit Xlen)) (Some (SyntaxConst (ConstBit pcInit))));
+                (@^"isWfi", existT RegInitValT (SyntaxKind Bool) (Some (SyntaxConst (ConstBool false))))
+              ] ++
+              @Fifo.Ifc.regs _ tokenFifo ++
+              @Fifo.Ifc.regs _ fetchAddrExceptionFifo ++
+              @Fifo.Ifc.regs _ fetchInstExceptionFifo ++
+              @Fifo.Ifc.regs _ decExecFifo ++
+              @Mem.Ifc.regs _ _ _ mem;
+         Pipeline.Ifc.regFiles
+           := @Fifo.Ifc.regFiles _ tokenFifo ++
+              @Fifo.Ifc.regFiles _ fetchAddrExceptionFifo ++
+              @Fifo.Ifc.regFiles _ fetchInstExceptionFifo ++
+              @Fifo.Ifc.regFiles _ decExecFifo ++
+              @Mem.Ifc.regFiles _ _ _ mem;
+         Pipeline.Ifc.tokenStartRule                := tokenStartRule;
+         Pipeline.Ifc.mmuSendReqRule                := Mem.Ifc.mmuSendReqRule mem;
+         Pipeline.Ifc.sendPcRule                    := sendPcRule;
+         Pipeline.Ifc.transferMmuFetchExceptionRule := transferMmuFetchExceptionRule;
+         Pipeline.Ifc.routerPollRules               := Mem.Ifc.routerPollRules mem;
+         Pipeline.Ifc.responseToFetcherRule         := Mem.Ifc.responseToFetcherRule mem;
+         Pipeline.Ifc.fetcherTransferRule           := Mem.Ifc.fetcherTransferRule mem;
+         Pipeline.Ifc.fetcherNotCompleteDeqRule     := Mem.Ifc.fetcherNotCompleteDeqRule mem;
+         Pipeline.Ifc.decodeExecRule                := decodeExecRule;
+         Pipeline.Ifc.commitRule                    := commitRule;
+         Pipeline.Ifc.arbiterResetRule              := Mem.Ifc.arbiterResetRule mem;
+       |}.
+
+End Impl.
