Pipeline/Mem/Impl.v
@@ -1,0 +1,291 @@
+Require Import Kami.AllNotations.
+
+Require Import ProcKami.MemRegion.
+Require Import ProcKami.MemOps.
+Require Import ProcKami.MemOpsFuncs.
+
+Require Import StdLibKami.RegArray.Ifc.
+Require Import StdLibKami.RegArray.Impl.
+
+Require Import StdLibKami.Fifo.Ifc.
+Require Import StdLibKami.Fifo.Impl.
+
+Require Import StdLibKami.FreeList.Ifc.
+Require Import StdLibKami.FreeList.Array.
+
+Require Import StdLibKami.Fetcher.Ifc.
+Require Import StdLibKami.Fetcher.Impl.
+
+Require Import StdLibKami.CompletionBuffer.Ifc.
+Require Import StdLibKami.CompletionBuffer.Impl.
+
+Require Import ProcKami.Pipeline.Mem.Mmu.Ifc.
+Require Import ProcKami.Pipeline.Mem.Mmu.Impl.
+
+Require Import StdLibKami.ReplacementPolicy.Ifc.
+Require Import StdLibKami.ReplacementPolicy.PseudoLru.
+
+Require Import StdLibKami.Cam.Ifc.
+Require Import StdLibKami.Cam.Impl.
+
+Require Import StdLibKami.Arbiter.Ifc.
+Require Import StdLibKami.Arbiter.Impl.
+
+Require Import StdLibKami.Router.Ifc.
+Require Import StdLibKami.Router.Impl.
+
+Require Import ProcKami.Pipeline.Decoder.
+
+Require Import ProcKami.Pipeline.Mem.PmaPmp.
+
+Require Import ProcKami.Pipeline.Mem.Ifc.
+
+Require Import ProcKami.FU.
+Require Import ProcKami.Device.
+
+Section Impl.
+  Context {procParams : ProcParams}.
+  Context (deviceTree : @DeviceTree procParams).
+  Context {memParams: Mem.Ifc.Params}.
+  
+  Context (memCallback: forall ty, ty (@MemResp _ memParams) -> ActionT ty Void).
+
+  Local Open Scope kami_expr.
+  Local Open Scope kami_action.
+
+  Local Definition fetcherParams :=
+    {|
+      Fetcher.Ifc.name       := @^"fetcher";
+      Fetcher.Ifc.size       := Nat.pow 2 (@fetcherLgSize memParams);
+      Fetcher.Ifc.memReqK    := PAddrDevOffset deviceTree;
+      Fetcher.Ifc.vAddrSz    := Xlen;
+      Fetcher.Ifc.compInstSz := FU.CompInstSz;
+      Fetcher.Ifc.immResK    := Void;
+      Fetcher.Ifc.finalErrK  := Bool;
+      Fetcher.Ifc.isCompressed
+      := fun ty (inst : Bit FU.CompInstSz @# ty)
+         => isInstCompressed inst;
+      Fetcher.Ifc.isImmErr := (fun _ _ => $$false);
+      Fetcher.Ifc.isFinalErr := (fun ty (finalErr: Bool @# ty) => finalErr)
+    |}.
+
+  Local Definition fetcher
+    : @Fetcher.Ifc.Ifc fetcherParams.
+  refine (@Fetcher.Impl.impl
+            fetcherParams
+            (@Fifo.Impl.impl _ {| Fifo.Impl.sizePow2 := _;
+                                  Fifo.Impl.regArray := RegArray.Impl.impl
+                               |})).
+  abstract (simpl; f_equal; rewrite Nat.log2_up_pow2; try lia).
+  Defined.
+
+  Local Definition completionBufferParams :=
+    {|
+      CompletionBuffer.Ifc.name      := @^"completionBuffer";
+      CompletionBuffer.Ifc.size      := Nat.pow 2 (@completionBufferLgSize memParams);
+      CompletionBuffer.Ifc.inReqK    := PAddrDevOffsetVAddr deviceTree;
+      CompletionBuffer.Ifc.outReqK   := PAddrDevOffset deviceTree;
+      CompletionBuffer.Ifc.storeReqK := FU.VAddr;
+      CompletionBuffer.Ifc.immResK   := Void;
+      CompletionBuffer.Ifc.resK      := Maybe FU.Inst;
+      CompletionBuffer.Ifc.inReqToOutReq
+      := fun ty req
+         => (STRUCT {
+                 "dtag" ::= req @% "memReq" @% "dtag";
+                 "offset" ::= ZeroExtendTruncLsb PAddrSz ({< ZeroExtendTruncMsb (PAddrSz - 2) (req @% "memReq" @% "offset"),
+                                                           $$(natToWord 2 0) >});
+                 "paddr" ::= ZeroExtendTruncLsb PAddrSz ({< ZeroExtendTruncMsb (PAddrSz - 2) (req @% "memReq" @% "paddr"),
+                                                           $$(natToWord 2 0) >})
+            })%kami_expr;
+      CompletionBuffer.Ifc.inReqToStoreReq
+      := fun ty req
+         => (req @% "vaddr")%kami_expr;
+      CompletionBuffer.Ifc.isError
+      := fun ty _ => $$false
+    |}.
+  
+  Local Definition completionBuffer
+    :  CompletionBuffer.Ifc.Ifc
+    := @CompletionBuffer.Impl.impl
+         completionBufferParams
+         {|
+           storeArray := @RegArray.Impl.impl _;
+           resArray   := @RegArray.Impl.impl _;
+           freeList   := @FreeList.Array.impl _
+         |}.
+
+  Local Definition mmu : Mmu.Ifc.Ifc deviceTree :=
+    @Mmu.Impl.impl _ deviceTree
+                   {| Mmu.Ifc.name := @^"mmu";
+                      Mmu.Ifc.lgPageSz := LgPageSz;
+                      Mmu.Ifc.maxVpnSz := vm_mode_max_vpn_size |}
+                      
+                   (@Cam.Impl.impl _ {|
+                                     Cam.Impl.size      := @tlbSize memParams;
+                                     Cam.Impl.policy    := ReplacementPolicy.PseudoLru.impl
+                                   |}).
+
+  Local Definition arbiterClients
+    :  list (Client (Maybe Data)).
+  refine [
+      (* memory unit client *)
+      {| clientTagSz := memUnitTagLgSize;
+         clientHandleRes := memCallback
+      |} ;
+      
+      (* MMU client *)
+      {| clientTagSz := 0;
+         clientHandleRes ty res := (LET res : Maybe FU.Data <- #res @% "res";
+                                    @Mmu.Ifc.callback _ deviceTree _ mmu _ res)%kami_action |};
+      (* Fetch Client *)                                                                                 
+      {| clientTagSz := @completionBufferLgSize memParams;
+         clientHandleRes ty
+                         (res: ty (STRUCT_TYPE { "tag" :: Bit _;
+                                                 "res" :: Maybe Data }))
+         := (LET inst: Maybe FU.Inst
+                       <- STRUCT { "valid" ::= #res @% "res" @% "valid" ;
+                                   "data"  ::= ZeroExtendTruncLsb FU.InstSz (#res @% "res" @% "data") };
+             LET fullRes: STRUCT_TYPE { "tag" :: Bit _;
+                                        "res" :: Maybe FU.Inst }
+                          <- STRUCT { "tag" ::= castBits _ (#res @% "tag");
+                                      "res" ::= #inst};
+             @CompletionBuffer.Ifc.callback _ completionBuffer ty fullRes)%kami_action |}
+    ].
+  abstract (simpl; rewrite Nat.log2_up_pow2; try lia).
+  Defined.
+
+  Local Definition arbiterParams :=
+    {|
+      Arbiter.Ifc.name    := @^"arbiter";
+      Arbiter.Ifc.inReqK  := @MemReq _ deviceTree;
+      Arbiter.Ifc.immResK := Void;
+      Arbiter.Ifc.isError := fun ty _ => Const ty false
+    |}.
+  
+  Local Definition arbiter
+    :  @Arbiter.Ifc.Ifc _ {| clientList := arbiterClients |}
+    := @Arbiter.Impl.impl arbiterParams _.
+
+  Definition ArbiterTag := Arbiter.Ifc.Tag {| clientList :=  arbiterClients |}.
+
+  Local Definition deviceIfcs := map (fun d => deviceIfc d ArbiterTag) (ProcKami.Device.devices deviceTree).
+
+  Local Definition routerParams := {|
+                                    Router.Ifc.name := @^"devRouter";
+                                    Router.Ifc.devices := deviceIfcs
+                                  |}.
+  
+  Local Definition router :=
+    @Router.Impl.impl routerParams.
+
+  Local Definition ArbiterOutReq := STRUCT_TYPE { "tag" :: ArbiterTag;
+                                                  "req" :: @MemReq _ deviceTree }.
+
+  Local Definition cbReqToArbiterReq ty (inReq: @CompletionBuffer.Ifc.OutReq completionBufferParams @# ty):
+    @Arbiter.Ifc.ClientReq arbiterParams (@completionBufferLgSize memParams) @# ty.
+  refine (
+    let req := (inReq @% "outReq") in
+    let reqStruct := STRUCT { "dtag" ::= req @% "dtag" ;
+                              "offset" ::= req @% "offset" ;
+                              "paddr" ::= req @% "paddr" ;
+                              "memOp" ::= getMemOpCode memOps _ Lw ;
+                              "data" ::= $$ (getDefaultConst Data) } in
+    STRUCT { "tag" ::= castBits _ (inReq @% "tag");
+             "req" ::= reqStruct }).
+  abstract (simpl; rewrite Natlog2_up_pow2; auto).
+  Defined.
+  
+  Local Definition arbiterReqToRouterReq ty (req: ty ArbiterOutReq): @Router.Ifc.OutReq routerParams @# ty.
+  refine (
+    let deviceInReq : Device.Req ArbiterTag @# ty := STRUCT { "tag" ::= #req @% "tag" ;
+                                                              "memOp" ::= #req @% "req" @% "memOp" ;
+                                                              "offset" ::= #req @% "req" @% "offset" ;
+                                                              "data" ::= #req @% "req" @% "data" } in
+    STRUCT { "dtag" ::= castBits _ (#req @% "req" @% "dtag") ;
+             "req" ::= deviceInReq}).
+  abstract (unfold numDevices; simpl; unfold deviceIfcs; rewrite map_length; auto).
+  Defined.
+  
+  
+  Local Definition routerSendReq ty (req: ty ArbiterOutReq): ActionT ty (Maybe Void) :=
+    LET inReq <- arbiterReqToRouterReq ty req;
+    LETA ret <- @Router.Ifc.sendReq _ router ty inReq;
+    Ret ((STRUCT { "valid" ::= #ret ;
+                   "data" ::= $$(getDefaultConst Void) }): Maybe Void @# ty).
+
+  Local Definition fetcherSendReq ty (req: ty Fetcher.Ifc.OutReq) :=
+    @Fetcher.Ifc.sendAddr
+      _ fetcher
+      (@CompletionBuffer.Ifc.sendReq
+         _ completionBuffer
+         (fun ty inReq2 =>
+            LET inReqFinal <- cbReqToArbiterReq #inReq2;
+            @Arbiter.Ifc.sendReq _ _ arbiter routerSendReq (Fin.FS (Fin.FS Fin.F1)) ty inReqFinal)
+      ) ty req.
+
+  Local Definition mmuSendReqRule ty: ActionT ty Void :=
+    @Mmu.Ifc.sendReqRule
+      _ _ _ mmu
+      (fun ty req =>
+         LET reqFinal: @Arbiter.Ifc.ClientReq arbiterParams 0 <- STRUCT { "tag" ::= $0;
+                                                                          "req" ::= #req };
+         LETA retVal <- @Arbiter.Ifc.sendReq _ _ arbiter routerSendReq (Fin.FS Fin.F1) ty reqFinal;
+         Ret (#retVal @% "valid")) ty.
+
+  Local Definition memSendReq ty (req: ty (MemUnitMemReq deviceTree)): ActionT ty Bool :=
+    LETA retVal <- @Arbiter.Ifc.sendReq _ _ arbiter routerSendReq Fin.F1 ty req;
+    Ret (#retVal @% "valid").
+
+  Local Definition responseToFetcherRule ty: ActionT ty Void :=
+    @CompletionBuffer.Ifc.callbackRule _ completionBuffer (fun ty resp =>
+                                                             LET fetcherResp: (@Fetcher.Ifc.InRes fetcherParams) <- STRUCT { "vaddr" ::= #resp @% "storeReq" ;
+                                                                                                                             "immRes" ::= #resp @% "immRes" ;
+                                                                                                                             "error" ::= !(#resp @% "res" @% "valid") ;
+                                                                                                                             "inst" ::= #resp @% "res" @% "data" };
+                                                             @Fetcher.Ifc.callback _ fetcher _ fetcherResp) ty.
+  Definition impl
+    :  Mem.Ifc.Ifc deviceTree
+    := {| Mem.Ifc.regs :=
+            ((Fetcher.Ifc.regs fetcher)
+               ++ CompletionBuffer.Ifc.regs completionBuffer
+               ++ Mmu.Ifc.regs mmu
+               ++ Arbiter.Ifc.regs arbiter
+               ++ Router.Ifc.regs router) ;
+
+          Mem.Ifc.regFiles :=
+            ((Fetcher.Ifc.regFiles fetcher)
+               ++ CompletionBuffer.Ifc.regFiles completionBuffer
+               ++ Mmu.Ifc.regFiles mmu
+               ++ Arbiter.Ifc.regFiles arbiter
+               ++ Router.Ifc.regFiles router) ;
+
+          fetcherIsFull := @Fetcher.Ifc.isFull _ fetcher;
+          Mem.Ifc.fetcherSendAddr := fetcherSendReq;
+          fetcherDeq := @Fetcher.Ifc.deq _ fetcher;
+          fetcherFirst := @Fetcher.Ifc.first _ fetcher;
+
+          fetcherClearTop := @Fetcher.Ifc.clearTop _ fetcher;
+          fetcherClear := @Fetcher.Ifc.clear _ fetcher;
+
+          fetcherNotCompleteDeqRule := @Fetcher.Ifc.notCompleteDeqRule _ fetcher;
+          fetcherTransferRule := @Fetcher.Ifc.transferRule _ fetcher;
+
+          Mem.Ifc.responseToFetcherRule := responseToFetcherRule;
+
+          memTranslate := Mmu.Ifc.memTranslate mmu;
+
+          mmuReadException := Mmu.Ifc.readException mmu;
+          mmuClearException := Mmu.Ifc.clearException mmu;
+
+          Mem.Ifc.mmuSendReqRule := mmuSendReqRule;
+
+          sendMemUnitMemReq := memSendReq;
+
+          arbiterResetRule := @Arbiter.Ifc.resetRule _ _ arbiter;
+
+          routerPollRules := @Router.Ifc.pollRules _ router (@Arbiter.Ifc.callback _ _ arbiter);
+       |}.
+
+  Local Close Scope kami_action.
+  Local Close Scope kami_expr.
+End Impl.
