Pipeline/Mem/PmaPmp.v
@@ -1,0 +1,145 @@
+Require Import Kami.AllNotations.
+
+Require Import ProcKami.FU.
+Require Import ProcKami.Device.
+Require Import ProcKami.MemOps.
+Require Import ProcKami.MemOpsFuncs.
+Require Import ProcKami.MemRegion.
+
+Require Import ProcKami.Pipeline.Mem.Pmp.
+
+Section PmaPmp.
+  Context {procParams: ProcParams}.
+
+  Context (deviceTree : @DeviceTree procParams).
+  Definition DeviceTag := Bit (Nat.log2_up (length (Device.devices deviceTree))).
+  
+  Local Open Scope kami_expr.
+  Local Open Scope kami_action.
+
+  Local Definition PmaSuccessPkt
+    := STRUCT_TYPE {
+         "width"      :: Bool;
+         "pma"        :: Bool;
+         "misaligned" :: Bool
+       }.
+
+
+  Local Definition mem_device_apply ty
+    (devs : list Device)
+    (devTag : DeviceTag @# ty)
+    (k : Kind)
+    (f : Device -> ActionT ty k)
+    :  ActionT ty k
+    := LETA result
+         <- utila_acts_find_pkt
+              (map
+                (fun dev : nat * Device
+                  => If devTag == $(fst dev)
+                       then
+                         LETA result <- f (snd dev);
+                         Ret (Valid #result : Maybe k @# ty)
+                       else Ret Invalid 
+                       as result;
+                     Ret #result)
+                (tag devs));
+       Ret (#result @% "data").
+
+  Local Definition checkPma ty
+    (dtag : DeviceTag @# ty)
+    (offset : FU.Offset @# ty)
+    (req_len : MemRqLgSize @# ty)
+    (access_type : AccessType @# ty)
+    :  ActionT ty PmaSuccessPkt 
+    := @mem_device_apply ty
+         (@ProcKami.Device.devices _ deviceTree)
+         dtag PmaSuccessPkt
+         (fun dev
+           => let acc_pmas f := (@Kor _ Bool) (map f (@pmas _ dev)) in
+              let width_match pma := req_len == $(pma_width pma) in
+              Ret (STRUCT {
+                  "width" ::= acc_pmas width_match;
+                  "pma"
+                    ::= acc_pmas
+                          (fun pma
+                            => width_match pma &&
+                               Switch access_type Retn Bool With {
+                                 ($VmAccessInst : AccessType @# ty)
+                                   ::= ($$(pma_executable pma) : Bool @# ty);
+                                 ($VmAccessLoad : AccessType @# ty)
+                                   ::= ($$(pma_readable pma) : Bool @# ty);
+                                 ($VmAccessSAmo : AccessType @# ty)
+                                   ::= ($$(pma_writeable pma) : Bool @# ty)
+                               });
+                  "misaligned"
+                    ::= acc_pmas
+                         (fun pma
+                           => width_match pma &&
+                              (isAligned offset req_len || 
+                               $$(pma_misaligned pma)))
+                } : PmaSuccessPkt @# ty)).
+
+
+  Local Definition DTagOffset := STRUCT_TYPE { "dtag" :: DeviceTag;
+                                               "offset" :: FU.Offset }.
+
+  Local Definition getDTagOffset ty
+    (addr : PAddr @# ty)
+    :  ActionT ty (Maybe DTagOffset)
+    := @memRegionApply
+         _
+         (length (ProcKami.Device.devices deviceTree))
+         ty DTagOffset addr
+         (fun region (offset: Offset @# ty)
+            =>
+              LET tagOffset
+                <- match mem_region_device region with
+                   | None => ($$ (getDefaultConst DTagOffset))
+                   | Some devTag
+                     => (STRUCT {
+                             "dtag" ::= $(proj1_sig (to_nat devTag));
+                             "offset" ::= offset
+                           } : DTagOffset @# ty)
+                   end;
+              Ret #tagOffset)
+         (memRegions (memTable _)).
+
+  Definition getDTagOffsetPmaPmpError ty
+             (accessType: AccessType @# ty)
+             (memOp: MemOpCode @# ty)
+             (mode: PrivMode @# ty)
+             (addr: PAddr @# ty)
+    :  ActionT ty (Pair (Maybe DTagOffset) MemErrorPkt)
+    := LETA size
+         :  MemRqLgSize
+         <- applyMemOp
+              memOps
+              (fun memOp
+                => Ret ($(memOpSize memOp) : MemRqLgSize @# ty))
+              memOp;
+       LETA pmp_result
+         :  Bool
+         <- checkPmp
+              accessType
+              mode
+              addr
+              #size;
+       LETA dTagOffset: Maybe DTagOffset <- getDTagOffset addr;
+       LETA pma_result
+         :  PmaSuccessPkt
+         <- checkPma
+              (#dTagOffset @% "data" @% "dtag")
+              (#dTagOffset @% "data" @% "offset")
+              #size
+              accessType;
+       LET err_pkt : MemErrorPkt
+         <- STRUCT {
+              "pmp"        ::= !#pmp_result;
+              "width"      ::= !(#pma_result @% "width");
+              "pma"        ::= !(#pma_result @% "pma");
+              "misaligned" ::= !(#pma_result @% "misaligned")
+            } : MemErrorPkt @# ty;
+       LET ret : Pair (Maybe DTagOffset) MemErrorPkt <- STRUCT { "fst" ::= #dTagOffset;
+                                                                 "snd" ::= #err_pkt };
+       Ret #ret.
+End PmaPmp.
