Pipeline/RegWriter.v
@@ -1,9 +1,12 @@
 Require Import Kami.AllNotations.
+
 Require Import ProcKami.FU.
+
+
 Import ListNotations.
 
 Section RegWriter.
-  Context `{procParams: ProcParams}.
+  Context {procParams: ProcParams}.
   Variable ty: Kind -> Type.
 
   Local Open Scope kami_action.
@@ -14,14 +17,17 @@ Section RegWriter.
     (reg_id : RegId @# ty)
     (data : Data @# ty)
     :  ActionT ty Void
-    := WriteRf @^"regWrite" (reg_id : RegIdWidth ; xlen_sign_extend Xlen xlen data : Bit Xlen);
-       System [
-         DispString _ " Reg Write Wrote ";
-         DispHex data;    
-         DispString _ " to register ";
-         DispHex reg_id;
-         DispString _ "\n"
-       ]%list;
+    := If reg_id != $0
+         then
+           WriteRf @^"regWrite" (reg_id : RegIdWidth ; xlen_sign_extend Xlen xlen data : Bit Xlen);
+           System [
+             DispString _ " Reg Write Wrote ";
+             DispHex data;    
+             DispString _ " to register ";
+             DispHex reg_id;
+             DispString _ "\n"
+           ]%list;
+         Retv;
        Retv.
 
   Definition reg_writer_write_freg
@@ -38,7 +44,15 @@ Section RegWriter.
        ]%list;
        Retv.
 
-  Close Scope kami_expr.
-  Close Scope kami_action.
+  Definition reg_writer_write_fflags
+    (data : Data @# ty)
+    :  ActionT ty Void
+    := Write @^"fflags"
+         :  FflagsValue
+         <- unsafeTruncLsb FflagsWidth data;
+       Retv.
+
+  Local Close Scope kami_expr.
+  Local Close Scope kami_action.
 
 End RegWriter.
