RiscvIsaSpec/Insts/Fpu/FMac.v
@@ -137,21 +137,14 @@ Section Fpu.
                                "tag"  ::= Const ty (natToWord RoutingTagSz FflagsTag);
                                "data" ::= ((csr (#sem_out_pkt @% "muladd_out" @% "exceptionFlags")) : Bit Rlen @# ty)
                                  });
-         LETC fstVal <- (STRUCT {
-                       "val1"
-                         ::= Valid #val1;
-                       "val2"
-                         ::= Valid #val2;
-                       "memBitMask" ::= $$(getDefaultConst (Array Rlen_over_8 Bool));
-                       "taken?" ::= $$false;
-                       "aq" ::= $$false;
-                       "rl" ::= $$false;
-                       "fence.i" ::= $$false
-                     } : ExecUpdPkt @# ty);
+         LETC fstVal
+           :  ExecUpdPkt
+           <- (noUpdPkt ty)
+                @%["val1" <- (Valid #val1)]
+                @%["val2" <- (Valid #val2)];
          RetE
            (STRUCT {
-              "fst"
-                ::= #fstVal;
+              "fst" ::= #fstVal;
               "snd" ::= Invalid
             } : PktWithException ExecUpdPkt @# ty).
   End ty.
