RiscvIsaSpec/Insts/Fpu/FMv.v
@@ -22,49 +22,49 @@ Section Fpu.
 
   Open Scope kami_expr.
 
+  Definition FMvInputType
+    :  Kind
+    := STRUCT_TYPE {
+         "isInt" :: Bool;
+         "data"  :: Data
+       }.
+
+  Definition FMvOutput
+    (ty : Kind -> Type)
+    (resultExpr : FMvInputType ## ty)
+    :  PktWithException ExecUpdPkt ## ty
+    := LETE result <- resultExpr;
+       RetE (STRUCT {
+         "fst"
+           ::= (noUpdPkt ty)
+                 @%["val1"
+                     <- Valid (STRUCT {
+                          "tag"
+                            ::= IF #result @% "isInt"
+                                  then $IntRegTag
+                                  else $FloatRegTag
+                                  : Bit RoutingTagSz @# ty;
+                          "data"
+                            ::= IF #result @% "isInt"
+                                  then
+                                    SignExtendTruncLsb Rlen
+                                      (ZeroExtendTruncLsb
+                                        fpu_len
+                                        (#result @% "data"))
+                                  else
+                                    OneExtendTruncLsb Rlen
+                                      (ZeroExtendTruncLsb
+                                        fpu_len
+                                        ((#result @% "data")))
+                        }) : Maybe RoutedReg @# ty];
+         "snd" ::= Invalid
+       } : PktWithException ExecUpdPkt @# ty).
+
   Definition FMv
     :  FUEntry
     := {|
          fuName := append "fmv" fpu_suffix;
-         fuFunc
-           := fun ty (sem_in_pkt : Pair Bool (Bit Rlen) ## ty)
-                => LETE inp <- sem_in_pkt;
-                   LETC isInt <- #inp @% "fst";
-                   LETC val1 <- ((STRUCT {
-                                             "tag"
-                                               ::= (IF #isInt
-                                                      then $IntRegTag
-                                                      else $FloatRegTag: Bit RoutingTagSz @# ty);
-                                             "data"
-                                               ::= (IF #isInt
-                                                      then SignExtendTruncLsb
-                                                             Rlen
-                                                             (ZeroExtendTruncLsb
-                                                               fpu_len
-                                                               ((#inp @% "snd") : Bit Rlen @# ty))
-                                                      else OneExtendTruncLsb
-                                                             Rlen
-                                                             (ZeroExtendTruncLsb
-                                                               fpu_len
-                                                               ((#inp @% "snd") : Bit Rlen @# ty)))
-                                    }: RoutedReg @# ty));
-                   LETC fstVal <-  (STRUCT {
-                                 "val1"
-                                   ::= Valid #val1;
-                                 "val2" ::= @Invalid ty _;
-                                 "memBitMask" ::= $$(getDefaultConst (Array Rlen_over_8 Bool));
-                                 "taken?" ::= $$false;
-                                 "aq" ::= $$false;
-                                 "rl" ::= $$false;
-                                 "fence.i" ::= $$false
-                                            
-                               } : ExecUpdPkt @# ty);
-                   RetE
-                     (STRUCT {
-                        "fst"
-                          ::= #fstVal;
-                        "snd" ::= Invalid
-                      } : PktWithException ExecUpdPkt @# ty);
+         fuFunc := fun ty => id;
          fuInsts
            := [
                 {|
@@ -85,13 +85,13 @@ Section Fpu.
                     := fun ty (cfg_pkt : ContextCfgPkt @# ty) context_pkt_expr
                          => LETE inp <- context_pkt_expr;
                             LETC ret
-                              :  Pair Bool (Bit Rlen)
+                              :  FMvInputType
                               <- STRUCT {
-                                   "fst" ::= $$true;
-                                   "snd" ::= #inp @% "reg1"
+                                   "isInt" ::= $$true;
+                                   "data"  ::= #inp @% "reg1"
                                  };
                             RetE #ret;
-                  outputXform := fun _ => id;
+                  outputXform := FMvOutput;
                   optMemParams := None;
                   instHints := falseHints<|hasFrs1 := true|><|hasRd := true|> 
                 |};
@@ -113,13 +113,13 @@ Section Fpu.
                     := fun ty (cfg_pkt : ContextCfgPkt @# ty) context_pkt_expr
                          => LETE inp <- context_pkt_expr;
                             LETC ret
-                              :  Pair Bool (Bit Rlen)
+                              :  FMvInputType
                               <- STRUCT {
-                                   "fst" ::= $$false;
-                                   "snd" ::= #inp @% "reg1"
+                                   "isInt" ::= $$false;
+                                   "data"  ::= #inp @% "reg1"
                                  };
                                  RetE #ret;
-                  outputXform := fun _ => id;
+                  outputXform := FMvOutput;
                   optMemParams := None;
                   instHints := falseHints<|hasRs1 := true|><|hasFrd := true|> 
                 |}
